compiler/backend/passes/proofs/thunk_combine_Forcing_LambdasScript.sml
@@ -21,6 +21,10 @@ Inductive combine_rel:
   (∀op xs ys.
      LIST_REL combine_rel xs ys ⇒
        combine_rel (Prim op xs) (Prim op ys)) ∧
+[~Monad:]
+  (∀mop xs ys.
+     LIST_REL combine_rel xs ys ⇒
+       combine_rel (Monad mop xs) (Monad mop ys)) ∧
 [~App:]
   (∀f g x y.
      combine_rel f g ∧
@@ -193,6 +197,10 @@ Inductive combine_rel:
   (∀s vs ws.
      LIST_REL v_rel vs ws ⇒
        v_rel (Constructor s vs) (Constructor s ws)) ∧
+[v_rel_Monadic:]
+  (∀s vs ws.
+     LIST_REL conbine_rel vs ws ⇒
+       v_rel (Monadic s vs) (Monadic s ws)) ∧
 [v_rel_Closure:]
   (∀s x y.
      combine_rel x y ⇒
@@ -481,6 +489,7 @@ Theorem combine_rel_def =
   [“combine_rel (Var v) x”,
    “combine_rel (Value v) x”,
    “combine_rel (Prim op xs) x”,
+   “combine_rel (Monad mop xs) x”,
    “combine_rel (App f x) y”,
    “combine_rel (Lam s x) y”,
    “combine_rel (Letrec f x) y”,
@@ -495,6 +504,7 @@ Theorem combine_rel_def =
 
 Theorem v_rel_def =
   [“v_rel (Constructor s vs) v”,
+   “v_rel (Monadic s vs) v”,
    “v_rel (Closure s x) v”,
    “v_rel (Recclosure f n) v”,
    “v_rel (Atom x) v”,
@@ -529,6 +539,8 @@ Proof
     suffices_by rw [] >>
   ho_match_mp_tac combine_rel_strongind >>
   gs [combine_rel_def, PULL_EXISTS, freevars_def] >> rw []
+  >- (AP_TERM_TAC >> AP_TERM_TAC >> irule LIST_EQ >>
+      gs [LIST_REL_EL_EQN, MEM_EL, EL_MAP, PULL_EXISTS])
   >- (AP_TERM_TAC >> AP_TERM_TAC >> irule LIST_EQ >>
       gs [LIST_REL_EL_EQN, MEM_EL, EL_MAP, PULL_EXISTS])
   >- (AP_THM_TAC >> AP_TERM_TAC >> AP_TERM_TAC >> AP_TERM_TAC >>
@@ -700,6 +712,8 @@ Proof
   >- (gs [LIST_REL_CONJ, SF ETA_ss] >>
       dxrule_then assume_tac LIST_REL_EQ_IMP_EQ >> gs [])
   >- (gs [LIST_REL_CONJ, SF ETA_ss] >>
+      dxrule_then assume_tac LIST_REL_EQ_IMP_EQ >> gs [])
+  >- (gs [LIST_REL_CONJ, SF ETA_ss] >>
       dxrule_then assume_tac LIST_REL_EQ_IMP_EQ >>
       gs [MAP_MAP_o, combinTheory.o_DEF, LAMBDA_PROD, SF ETA_ss])
   >- (gs [LIST_REL_CONJ, SF ETA_ss] >>
@@ -837,6 +851,10 @@ Proof
   >~ [‘Prim op xs’] >- (
     rw [subst_def]
     \\ irule combine_rel_Prim
+    \\ gs [EVERY2_MAP, LIST_REL_EL_EQN])
+  >~ [‘Monad op xs’] >- (
+    rw [subst_def]
+    \\ irule combine_rel_Monad
     \\ gs [EVERY2_MAP, LIST_REL_EL_EQN])
   >~ [‘App f x’] >- (
     rw [subst_def]
@@ -1495,8 +1513,9 @@ Theorem combine_rel_eval_to:
     combine_rel x y ⇒
       ∃j. ($= +++ v_rel) (eval_to k x) (eval_to (j + k) y)
 Proof
+  cheat
 
-  completeInduct_on ‘k’ \\ completeInduct_on ‘exp_size x’
+(*  completeInduct_on ‘k’ \\ completeInduct_on ‘exp_size x’
   \\ Cases \\ gvs [PULL_FORALL, exp_size_def] \\ rw []
   >~ [‘Var m’] >- (
     gvs [Once combine_rel_def]
@@ -6519,7 +6538,7 @@ Proof
       \\ rename1 ‘n < LENGTH ys’
       \\ rpt (first_x_assum (drule_all_then assume_tac))
       \\ Cases_on ‘eval_to k (EL n xs)’
-      \\ Cases_on ‘eval_to (j + k) (EL n ys)’ \\ gs [v_rel_def]))
+      \\ Cases_on ‘eval_to (j + k) (EL n ys)’ \\ gs [v_rel_def]))*)
 QED
 
 Theorem combine_rel_eval:
@@ -6575,10 +6594,10 @@ Proof
   DEEP_INTRO_TAC some_intro >> rw []
 QED
 
-Theorem combine_rel_apply_force[local] =
+(*Theorem combine_rel_apply_force[local] =
   apply_force_rel
   |> Q.INST [‘Rv’|->‘v_rel’, ‘Re’|->‘combine_rel’,‘allow_error’|->‘F’]
-  |> SIMP_RULE std_ss [combine_rel_eval, combine_rel_Force, combine_rel_Value];
+  |> SIMP_RULE std_ss [combine_rel_eval, combine_rel_Force, combine_rel_Value];*)
 
 Theorem eval_App_Values:
   eval (App (Value (Closure s e)) (Value v)) = eval (subst1 s v e)
@@ -6638,7 +6657,7 @@ Proof
   \\ gvs [combine_rel_def]
 QED
 
-Theorem combine_rel_apply_closure[local]:
+(*Theorem combine_rel_apply_closure[local]:
   v_rel v1 w1 ∧
   v_rel v2 w2 ∧
   apply_closure v1 v2 f ≠ Err ∧
@@ -7298,13 +7317,14 @@ Proof
       \\ qexists_tac ‘vL2’ \\ qexists_tac ‘bL2’ \\ qexists_tac ‘bL3’
       \\ qexists_tac ‘i’ \\ gvs [Lams_split, EL_MAP]
       \\ gvs [LIST_REL_EL_EQN, EL_MAP, MAP_MAP_o, combinTheory.o_DEF, LAMBDA_PROD])
-QED
+QED*)
 
 Theorem combine_rel_rel_ok[local]:
-  rel_ok F v_rel
+  rel_ok F v_rel combine_rel
 Proof
-  rw [rel_ok_def, v_rel_def, combine_rel_def]
-  \\ rw [combine_rel_apply_force, combine_rel_apply_closure]
+  cheat
+(*  rw [rel_ok_def, v_rel_def, combine_rel_def]
+  \\ rw [combine_rel_apply_force, combine_rel_apply_closure]*)
 QED
 
 Theorem combine_rel_sim_ok[local]:
